theories/typing/uniq_array_util.v
@@ -29,19 +29,19 @@ Section uniq_array_util.
     by iMod (bor_combine with "LFT ξ ξl") as "$".
   Qed.
 
-  (* Lemma ty_own_proph_big_sepL_uniq_body {𝔄} (ty: type 𝔄) n (vπξil: vec _ n)
+  Lemma ty_own_proph_big_sepL_uniq_body {𝔄} (ty: type 𝔄) n (vπξil: vec _ n)
       d κ tid l κ' q E :
     ↑lftN ⊆ E → lft_ctx -∗ κ' ⊑ κ -∗ κ' ⊑ ty_lft ty -∗
     ([∗ list] i ↦ vπξi ∈ vπξil, uniq_body ty vπξi.1 vπξi.2 d κ tid (l +ₗ[ty] i)) -∗
     q.[κ'] ={E}=∗ |={E}▷=>^(S d) |={E}=>
       let ξl := vmap (λ vπξi, PrVar (𝔄 ↾ prval_to_inh vπξi.1) vπξi.2) vπξil in
-      ∃ζl q', ⌜vapply (vmap fst vπξil) ./ ζl⌝ ∗ q':+[ζl ++ ξl] ∗
-        (q':+[ζl ++ ξl] ={E}=∗
+      ∃ζll q', ⌜Forall2 ty.(ty_proph) (vmap fst vπξil) ζll⌝ ∗ q':+[mjoin ζll ++ ξl] ∗
+        (q':+[mjoin ζll ++ ξl] ={E}=∗
           ([∗ list] i ↦ vπξi ∈ vπξil, uniq_body ty vπξi.1 vπξi.2 d κ tid (l +ₗ[ty] i)) ∗
           q.[κ']).
   Proof.
     iIntros (?) "#LFT #In #In' uniqs κ'". iInduction vπξil as [|] "IH" forall (q l).
-    { iApply step_fupdN_full_intro. iIntros "!>!>". iExists [], 1%Qp.
+    { iApply step_fupdN_full_intro. iIntros "!>!>". iExists [], 1%Qp. simpl.
       do 2 (iSplit; [done|]). iIntros. by iFrame. }
     iDestruct "uniqs" as "[uniq uniqs]". iDestruct "κ'" as "[κ' κ'₊]"=>/=.
     iMod (ty_own_proph_uniq_body with "LFT In In' uniq κ'") as "Upd"; [done|].
@@ -51,13 +51,13 @@ Section uniq_array_util.
     iDestruct (proph_tok_combine with "ζl ζl'") as (?) "[ζζl Toζζl]".
     iDestruct (proph_tok_combine with "ξ ξl") as (?) "[ξl Toξl]".
     iDestruct (proph_tok_combine with "ζζl ξl") as (?) "[ζζξl Toζζξl]".
-    iExists _, _. iFrame "ζζξl". iSplit. { iPureIntro. by apply proph_dep_vec_S. }
+    iExists (_ :: _), _. simpl. iFrame "ζζξl". iSplit. { iPureIntro. constructor; done. }
     iIntros "ζζξl". iDestruct ("Toζζξl" with "ζζξl") as "[ζζl ξl]".
     iDestruct ("Toζζl" with "ζζl") as "[ζl ζl']".
-    iDestruct ("Toξl" with "ξl") as "[ξ ξl]".
-    iMod ("Touniq" with "[$ζl $ξ]") as "[$$]".
+    iDestruct ("Toξl" with "ξl") as "[[ξ _] ξl]".
+    iMod ("Touniq" with "[$ζl $ξ]") as "[$$]". done.
     by iMod ("Touniqs" with "[$ζl' $ξl]") as "[$$]".
-  Qed. *)
+  Qed.
 
   Lemma resolve_big_sepL_uniq_body {𝔄} (ty: type 𝔄) n (vπξil: vec _ n) d κ tid l E L q F :
     lctx_lft_alive E L κ → ↑lftN ∪ ↑prophN ⊆ F →
@@ -121,14 +121,14 @@ Section uniq_array_util.
     iMod "IH" as (?) "?". iModIntro. iExists (_:::_). iFrame.
   Qed.
 
-  Lemma uniq_proph_tok_vec {𝔄 n} (vπξil: vec (proph 𝔄 * _) n) d :
+  Lemma uniq_proph_tok_vec {𝔄 n} (vπξil: vec (proph 𝔄 * _) n) d (P: (proph 𝔄) → _) :
     ([∗ list] vπξi ∈ vπξil,
       let ξ := PrVar (𝔄 ↾ prval_to_inh vπξi.1) vπξi.2 in
-      .VO[ξ] vπξi.1 d ∗ .PC[ξ] vπξi.1 d) -∗
+      .VO[ξ] vπξi.1 d ∗ .PC[ξ, P] vπξi.1 d) -∗
     let ξl := map (λ vπξi, PrVar (𝔄 ↾ prval_to_inh vπξi.1) vπξi.2) vπξil in
     1:+[ξl] ∗ (1:+[ξl] -∗ [∗ list] vπξi ∈ vπξil,
       let ξ := PrVar (𝔄 ↾ prval_to_inh vπξi.1) vπξi.2 in
-      .VO[ξ] vπξi.1 d ∗ .PC[ξ] vπξi.1 d).
+      .VO[ξ] vπξi.1 d ∗ .PC[ξ, P] vπξi.1 d).
   Proof.
     iIntros "VoPcs". iInduction vπξil as [|] "IH". { iSplitL; by [|iIntros]. }
     iDestruct "VoPcs" as "[[Vo Pc] VoPcs]"=>/=.
@@ -137,24 +137,24 @@ Section uniq_array_util.
     iDestruct ("ToPc" with "ξ") as "$". iDestruct ("ToVoPcs" with "ξl") as "$".
   Qed.
 
-  (* Lemma proph_dep_prvars {𝔄 n} (vπξil: vec (proph 𝔄 * _) n) :
+  Lemma proph_dep_prvars {𝔄 n} (vπξil: vec (proph 𝔄 * _) n) :
     let ξl := map (λ vπξi, PrVar (𝔄 ↾ prval_to_inh vπξi.1) vπξi.2) vπξil in
     let vπl' := vmap (λ vπξi (π: proph_asn),
       π (PrVar (𝔄 ↾ prval_to_inh vπξi.1) vπξi.2): 𝔄) vπξil in
-    vapply vπl' ./ ξl.
+    vapply vπl' ./[𝔄] ξl.
   Proof.
     elim: vπξil; [done|]=>/= ????. apply (proph_dep_vec_S [_]); [|done].
     apply proph_dep_one.
-  Qed. *)
+  Qed.
 
-  (* Lemma merge_big_sepL_proph_ctrl_mt_ty_own {𝔄 n}
-      (vπl: vec _ n) ξil (ty: type 𝔄) d tid l :
+  Lemma merge_big_sepL_proph_ctrl_mt_ty_own {𝔄 n}
+      (vπl: vec _ n) ξil (ty: type 𝔄) d tid l:
     ⧖(S d) -∗
     ([∗ list] vπξi ∈ vzip vπl ξil,
-      .PC[PrVar (𝔄 ↾ prval_to_inh vπξi.1) vπξi.2] vπξi.1 d) -∗
+      .PC[PrVar (𝔄 ↾ prval_to_inh vπξi.1) vπξi.2, ty.(ty_proph)] vπξi.1 d) -∗
     ([∗ list] i ↦ vπ ∈ vπl, (l +ₗ[ty] i) ↦∗: ty.(ty_own) vπ d tid) -∗
     [∗ list] i ↦ vπξi ∈ vzip vπl ξil, ∃vπ' d', ⧖(S d') ∗
-      .PC[PrVar (𝔄 ↾ prval_to_inh vπξi.1) vπξi.2] vπ' d' ∗
+      .PC[PrVar (𝔄 ↾ prval_to_inh vπξi.1) vπξi.2, ty.(ty_proph)] vπ' d' ∗
       (l +ₗ[ty] i) ↦∗: ty.(ty_own) vπ' d' tid.
   Proof.
     iIntros "#⧖ Pcs ↦tys". iInduction vπl as [|] "IH" forall (l); inv_vec ξil=>//= ??.
@@ -167,17 +167,17 @@ Section uniq_array_util.
       (vπξil: vec _ n) (ty: type 𝔄) dex tid l :
     proph_ctx -∗ ⧖(S dex) -∗
     ([∗ list] i ↦ vπξi ∈ vπξil, ∃vπ' d', ⧖(S d') ∗
-      .PC[PrVar (𝔄 ↾ prval_to_inh vπξi.1) vπξi.2] vπ' d' ∗
+      .PC[PrVar (𝔄 ↾ prval_to_inh vπξi.1) vπξi.2, ty.(ty_proph)] vπ' d' ∗
       (l +ₗ[ty] i) ↦∗: ty.(ty_own) vπ' d' tid) -∗
     ∃wπl d, ⧖(S d) ∗
       ([∗ list] vπξiwπ ∈ vzip vπξil wπl,
-        (.$ PrVar (𝔄 ↾ prval_to_inh vπξiwπ.1.1) vπξiwπ.1.2) :== vπξiwπ.2) ∗
+        (.$ PrVar (𝔄 ↾ prval_to_inh vπξiwπ.1.1) vπξiwπ.1.2) :={ty.(ty_proph)}= vπξiwπ.2) ∗
       ([∗ list] i ↦ wπ ∈ wπl, (l +ₗ[ty] i) ↦∗: ty.(ty_own) wπ d tid).
   Proof.
     iIntros "#PROPH #⧖ex Pc↦tys". iInduction vπξil as [|] "IH" forall (l).
     { iExists [#], _. by iFrame "⧖ex"=>/=. }
     iDestruct "Pc↦tys" as "[(%&%& ⧖ & Pc & ↦ty) Pc↦tys]".
-    iDestruct (proph_ctrl_eqz with "PROPH Pc") as "Eqz".
+    iDestruct (proph_ctrl_eqz' with "PROPH Pc") as "Eqz".
     setoid_rewrite <-shift_loc_assoc_nat.
     iDestruct ("IH" with "Pc↦tys") as (??) "(⧖' & Eqzs & ↦tys)".
     iCombine "⧖ ⧖'" as "⧖". iExists (_:::_), _=>/=. iFrame "⧖ Eqz Eqzs".
@@ -186,16 +186,33 @@ Section uniq_array_util.
     - setoid_rewrite shift_loc_assoc_nat. do 6 f_equiv. apply ty_own_depth_mono. lia.
   Qed.
 
-  Lemma proph_eqz_prvars {𝔄 n} vπξil (wπl: vec (proph 𝔄) n) :
+  Lemma proph_eqz_prvars {𝔄 n} vπξil (wπl: vec (proph 𝔄) n) (P: (proph 𝔄) → _) :
     ([∗ list] vπξiwπ ∈ vzip vπξil wπl,
-      (.$ PrVar (𝔄 ↾ prval_to_inh vπξiwπ.1.1) vπξiwπ.1.2) :== vπξiwπ.2) -∗
+      (.$ PrVar (𝔄 ↾ prval_to_inh vπξiwπ.1.1) vπξiwπ.1.2) :={P}= vπξiwπ.2) -∗
     let vπl := vmap (λ vπξi (π: proph_asn),
       π (PrVar (𝔄 ↾ prval_to_inh vπξi.1) vπξi.2): 𝔄) vπξil in
-    vapply vπl :== vapply wπl.
+    vapply vπl :={λ vπ ξl, exists ξll, ξl = mjoin ξll /\ Forall2 P (vfunsep vπ) ξll}= vapply wπl.
   Proof.
     iIntros "Eqzs". iInduction vπξil as [|] "IH"; inv_vec wπl=>/= *.
     { iApply proph_eqz_refl. }
     iDestruct "Eqzs" as "[Eqz Eqzs]". iDestruct ("IH" with "Eqzs") as "Eqz'".
-    iApply (proph_eqz_constr2 vcons' with "Eqz Eqz'").
-  Qed. *)
+    iApply proph_eqz_mono; [|iApply (proph_eqz_constr2 vcons' with "Eqz Eqz'")].
+    intros ?(?&->&?). inversion_clear H. eexists _, _, _, _.  intuition. fun_ext=>?/=. done. done. eexists _. done.
+  Qed.
+
+  Definition eq_rect_vec {A n m} (v: vec A n) (eq: n = m) := (eq_rect _ (λ n, vec A n) v _ eq).
+
+  Lemma eq_rect_vec_to_list {A} n m (v: vec A n) (eq: n = m): (vec_to_list (eq_rect_vec v eq)) = (vec_to_list v).
+  Proof. assert (eq' := eq). revert eq. rewrite -eq'. intros ?.  rewrite (eq_pi _ _ eq eq_refl). done. Qed.
+
+  Lemma proph_eqz_vec_to_list {𝔄 n} (vπl: (vec _ n)) (vπl': (vec _ n)) (P: (proph 𝔄) → _) :
+    vapply vπl :={λ vπ ξl, exists ξll, ξl = mjoin ξll /\ Forall2 P (vfunsep vπ) ξll}= vapply vπl' -∗
+    lapply vπl :={λ vπ ξl, exists aπl ξll, ξl = mjoin ξll /\ vπ = lapply aπl /\ Forall2 P aπl ξll}= lapply vπl'.
+  Proof.
+    iIntros "Eqz". rewrite -2! vec_to_list_apply. iApply proph_eqz_mono; [|iApply (proph_eqz_constr with "Eqz")].
+    intros ? (?&?&?&?&?). eexists (vapply (eq_rect_vec (list_to_vec x) _)). rewrite H0 vec_to_list_apply semi_iso' eq_rect_vec_to_list vec_to_list_to_vec.
+    intuition. eexists _. done. Unshelve. 
+    erewrite <- fmap_length. rewrite vec_to_list_apply /lapply in H0. erewrite <- (equal_f H0 inhabitant).
+    rewrite fmap_length vec_to_list_length. reflexivity.
+  Qed.
 End uniq_array_util.
